

① Name: Shivam Shekha

② Roll Number: shivam-ps2608mch135@iitp.ac.in.

Problem ①:-

Let  $P$ : Neeson is brave

$Q$ : Neeson is kind

i)  $(P \vee Q) \wedge (P \rightarrow \neg Q)$

$\rightarrow$  (Neeson is brave or Neeson is kind) and (if Neeson is brave then Neeson is not kind).

ii)  $(P \rightarrow Q) \wedge (Q \rightarrow P)$

$P \rightarrow Q$ : if Neeson is brave, then Neeson is kind

$Q \rightarrow P$ : if Neeson is kind, then Neeson is brave.

Therefore both are True or both are false, it is  $P \leftrightarrow Q$  (biconditional).

$\rightarrow$  (Neeson is kind if and only if Neeson is brave).

Problem ②:-

$A$ : The project is funded

$B$ : The team expands

$C$ : Productivity increases.

1. If the project is funded, then team will expand:  $A \rightarrow B$

2. If team expands, productivity increases:  $B \rightarrow C$

3. Productivity did not increase:  $\neg C$

CONCLUSION:  $\neg A$



10 milder

then  $A \rightarrow C$

$$(1,0,0) \in (1,0,0) \wedge (0,0,1) \quad \text{f. f. } \textcircled{1}$$

Now we have  $A \rightarrow C$  and  $\neg C$  Then  $\rightarrow A$

*[Faint handwritten notes at the bottom of the page]*

$$(\neg(p \wedge q)) \leftarrow (\neg p) \vee (\neg q) \quad (1)$$

① Some vegetarians do not like bitter gourd.

the thing is not

who is vegetarian and don't like bittergourd.

predicate form  $\exists x (Y(x) \wedge \neg L(x))$

There exists a bird that is not a bird

② maldar

$$(r \vee s) \leftarrow p \equiv (s \leftarrow p) \leftarrow r \leftarrow$$

2010-11-10

$$T \in \mathcal{P}(V) \rightarrow T \in \mathcal{P}(V) \rightarrow T \in \mathcal{P}(V)$$
[illegible][illegible]



### Problem 4:-

$B(x)$  :  $x$  is a bird,  $W(y)$  :  $y$  is a worm,  $E(x, y)$  :  $x$  eats  $y$ .

(i)  $\forall x \forall y (B(x) \wedge W(y) \rightarrow E(x, y))$

for any  $x$  and  $y$ , if  $x$  is a bird and  $y$  is a worm, then  $x$  eats  $y$ .

English Sentence :- "Every bird eats every worm".

(ii)  $\forall x \forall y (E(x, y) \rightarrow (B(x) \wedge W(y)))$

English :- Whenever something eats something, the eater is a bird and the thing eaten is a worm.

(iii)  $\exists x (B(x) \wedge \forall y (B(y) \rightarrow E(x, y)))$

C. there is atleast one bird  $x$  for every  $y$  such that if  $y$  is a bird  $x$  eats  $y$ .

English :- There exists a bird that eats every bird.

### Problem 5:-

$$\neg P \rightarrow (Q \rightarrow R) \equiv Q \rightarrow (P \vee R)$$

Solving with Truth Table:-

$P$	$Q$	$R$	$\neg P$	$Q \rightarrow R$	$\neg P \rightarrow (Q \rightarrow R)$	$P \vee R$	$Q \rightarrow (P \vee R)$
T	T	T	F	T	T	T	T
T	T	F	F	F	F	T	F
T	F	T	F	T	T	T	T
T	F	F	F	T	T	T	T
F	T	T	T	T	T	T	T
F	T	F	T	F	F	T	F
F	F	T	T	T	T	T	T
F	F	F	T	T	T	F	T

Therefore ! -  $\neg P \rightarrow (Q \rightarrow r) \equiv Q \rightarrow (P \vee r)$

Solving without Truth Table:

$$\text{L.H.S} = \neg P \rightarrow (Q \rightarrow r)$$

Step 1 :- Remove the inner Implication

$$Q \rightarrow r \equiv \neg Q \vee r$$

$$\text{so } \neg P \rightarrow (\neg Q \vee r)$$

Step 2 :- Remove the outer implication.

if  $a \rightarrow b \equiv \neg a \vee b$ , then.

$$\neg P \rightarrow (\neg Q \vee r) \equiv \neg(\neg P) \vee (\neg Q \vee r) \equiv P \vee (\neg Q \vee r)$$

Step 3 :- Associative law.

$$P \vee (\neg Q \vee r) \equiv \neg Q \vee (P \vee r)$$

$$\text{as } \neg Q \vee X \equiv Q \rightarrow X$$

$$\therefore \neg Q \vee (P \vee r) \equiv Q \rightarrow (P \vee r)$$

hence proved  $\neg P \rightarrow (Q \rightarrow r) \equiv Q \rightarrow (P \vee r)$

Problem 6:-  $(P \rightarrow Q) \wedge (R \rightarrow S); (Q \rightarrow T) \wedge (S \rightarrow U); \neg(T \wedge U) \therefore (P \rightarrow R) \Rightarrow \neg P$

1) Direct Method (True Column proof)

Statements

Reasons

1.  $(P \rightarrow Q) \wedge (R \rightarrow S)$

premise

2.  $(Q \rightarrow T) \wedge (S \rightarrow U)$

premise

3.  $\neg(T \wedge U)$

premise

4.  $P \rightarrow R$

premise

5.  $P \rightarrow Q$

from (1)

6.  $R \rightarrow S$

from (1)

7.  $Q \rightarrow T$

from (2)

8.  $S \rightarrow U$

from (2)

9.  $P \rightarrow T$

from (5, 7)

10.  $P \rightarrow S$

from (6, 8)

11.  $P \rightarrow U$

from (10, 9)

12.  $P \rightarrow (T \wedge U)$

from (9, 11) by conjunction

13.  $\neg P$

Modus Tollens (12, 3)

Therefore  $\neg P$ .



# 11) Indirect Method (Proof by Contradiction).

assume  $p$ .

## Statements

## Reasons

1.	$(p \rightarrow q) \wedge (r \rightarrow s)$	Implication premise
2.	$(q \rightarrow t) \wedge (s \rightarrow u)$	premise
3.	$\neg (t \wedge u)$	premise
4.	$p \rightarrow r$	premise
5.	Assume $p$	Assumption
6.	$p \rightarrow q$	from ①
7.	$r \rightarrow s$	from ①
8.	$q \rightarrow t$	from ②
9.	$s \rightarrow u$	from ②
10.	$r$	Modus Ponens (4, 5)
11.	$s$	Modus Ponens (7, 10)
12.	$u$	Modus Ponens (9, 11)
13.	$q$	Modus Ponens (6, 5)
14.	$t$	Modus Ponens (8, 13)
15.	$t \wedge u$	Conjunction (14, 12)
16.	Contradiction	from (3, 15)

$\therefore p$  leads to contradiction  $\neg p$ .

### Problem 7:-

SHOW  $\forall x (P(x) \rightarrow (Q(y) \wedge R(x)))$  and  $\exists x P(x) \Rightarrow Q(y) \wedge \exists x (R(x) \wedge P(x))$

Proof:-

1.  $\forall x (P(x) \rightarrow (Q(y) \wedge R(x)))$  (premise / given)
2.  $\exists x P(x)$  (premise / given)
3.  $P(a)$  (Existential Instantiation)
4.  $P(a) \rightarrow (Q(y) \wedge R(a))$
5.  $Q(y) \wedge R(a)$  (Modus Ponens) (from 3, 4)
6.  $Q(y)$  (from 5)
7.  $R(a)$  (from 5)
8.  $P(a) \wedge R(a)$  (Conjunction)
9.  $\exists x (P(x) \wedge R(x))$  (from 8)
10.  $Q(y) \wedge \exists x (P(x) \wedge R(x))$  (Conjunction) (combine 6, 9)

hence proved.